Prove compile_fn_preserves_aff_op

Wavelet/Compile/AffineOp.lean
@@ -12,8 +12,8 @@ open Semantics
 /-- Usage of a subset of operators is affine. -/
 inductive Expr.AffineInrOp [Arity Op₁] [Arity Op₂]
   : List Op₂ → Expr (Op₁ ⊕ Op₂) χ m n → Prop where
-  | aff_ret : AffineInrOp used (.ret vars)
-  | aff_tail : AffineInrOp used (.tail vars)
+  | aff_ret : AffineInrOp [] (.ret vars)
+  | aff_tail : AffineInrOp [] (.tail vars)
   | aff_op_inl
       {op : Op₁}
       {args : Vector χ (Arity.ι op)}
@@ -30,12 +30,14 @@ inductive Expr.AffineInrOp [Arity Op₁] [Arity Op₂]
       AffineInrOp used cont →
       AffineInrOp (op :: used) (.op (.inr op) args rets cont)
   | aff_br :
-      AffineInrOp used left →
-      AffineInrOp used right →
-      AffineInrOp used (.br cond left right)
+      AffineInrOp used₁ left →
+      AffineInrOp used₂ right →
+      used₁.Disjoint used₂ →
+      AffineInrOp (used₁ ++ used₂) (.br cond left right)
 
 def Fn.AffineInrOp [Arity Op₁] [Arity Op₂]
-  (fn : Fn (Op₁ ⊕ Op₂) χ V m n) : Prop := fn.body.AffineInrOp []
+  (fn : Fn (Op₁ ⊕ Op₂) χ V m n) : Prop :=
+  ∃ used, fn.body.AffineInrOp used
 
 def Prog.AffineInrOp [Arity Op]
   (prog : Prog Op χ V sigs) : Prop := ∀ i, (prog i).AffineInrOp
@@ -46,11 +48,20 @@ namespace Wavelet.Dataflow
 
 open Semantics
 
+def AtomicProcs.AffineInrOp
+  [Arity Op₁] [Arity Op₂]
+  (aps : AtomicProcs (Op₁ ⊕ Op₂) χ V)
+  (usedOps : List Op₂) : Prop
+  := ∀ {depOp inputs inputs' outputs outputs'},
+    .op (.inr depOp) inputs outputs ∈ aps →
+    .op (.inr depOp) inputs' outputs' ∈ aps →
+    inputs = inputs' ∧ outputs = outputs' ∧ depOp ∈ usedOps
+
 /-- Usage of a subset of operators is affine. -/
 def Proc.AffineInrOp
   [Arity Op₁] [Arity Op₂]
   (proc : Proc (Op₁ ⊕ Op₂) χ V m n) : Prop
-  := ∀ depOp inputs inputs' outputs outputs',
+  := ∀ {depOp inputs inputs' outputs outputs'},
     .op (.inr depOp) inputs outputs ∈ proc.atoms →
     .op (.inr depOp) inputs' outputs' ∈ proc.atoms →
     inputs = inputs' ∧ outputs = outputs'
@@ -61,6 +72,75 @@ namespace Wavelet.Compile
 
 open Semantics Seq Dataflow Fn
 
+/-- `compileExpr` preserves `AffineInrOp`. -/
+theorem compile_expr_preserves_aff_op
+  [Arity Op₁] [Arity Op₂]
+  [DecidableEq χ]
+  [InterpConsts V]
+  {expr : Expr (Op₁ ⊕ Op₂) χ m n}
+  (haff : expr.AffineInrOp usedOps)
+  : (compileExpr (V := V) hnz definedVars pathConds expr).AffineInrOp usedOps
+  := by
+  induction expr generalizing definedVars pathConds usedOps with
+  | ret => simp [compileExpr, AtomicProcs.AffineInrOp]
+  | tail => simp [compileExpr, AtomicProcs.AffineInrOp]
+  | op o args rets cont ih =>
+    cases o with
+    | inl op₁ =>
+      cases haff with | aff_op_inl haff =>
+      simp [compileExpr, AtomicProcs.AffineInrOp]
+      intros
+      rename_i hmem₁ hmem₂
+      exact ih (hnz := hnz) haff hmem₁ hmem₂
+    | inr op₂ =>
+      cases haff with | aff_op_inr hnot_mem haff =>
+      simp [compileExpr, AtomicProcs.AffineInrOp]
+      intros depOp
+      intros
+      rename_i hmem₁ hmem₂
+      cases hmem₁ <;> cases hmem₂
+      · rename_i hmem₁ hmem₂
+        have ⟨h₁, h₂, h₃⟩ := hmem₁
+        have ⟨_, h₂', h₃'⟩ := hmem₂
+        simp [← h₁] at hnot_mem
+        simp [hnot_mem]
+        have := HEq.trans h₂ h₂'.symm
+        simp at this
+        simp [this]
+        have := HEq.trans h₃ h₃'.symm
+        simp at this
+        simp [this]
+        assumption
+      · rename_i hmem₁ hmem₂
+        have := ih (hnz := hnz) haff hmem₂ hmem₂
+        simp [hmem₁.1] at this
+        exact False.elim (hnot_mem this)
+      · rename_i hmem₁ hmem₂
+        have := ih (hnz := hnz) haff hmem₁ hmem₁
+        simp [hmem₂.1] at this
+        exact False.elim (hnot_mem this)
+      · rename_i hmem₁ hmem₂
+        simp [ih (hnz := hnz) haff hmem₁ hmem₂]
+  | br cond left right ih₁ ih₂ =>
+    cases haff with | aff_br haff₁ haff₂ hdisj
+    simp [compileExpr, AtomicProcs.AffineInrOp, compileExpr.branchMerge]
+    intros
+    rename_i hmem₁ hmem₂
+    cases hmem₁ <;> cases hmem₂
+    · rename_i hmem₁ hmem₂
+      simp [ih₁ (hnz := hnz) haff₁ hmem₁ hmem₂]
+    · rename_i hmem₁ hmem₂
+      have ⟨_, _, h₁⟩ := ih₁ (hnz := hnz) haff₁ hmem₁ hmem₁
+      have ⟨_, _, h₂⟩ := ih₂ (hnz := hnz) haff₂ hmem₂ hmem₂
+      exact False.elim (hdisj h₁ h₂)
+    · rename_i hmem₂ hmem₁
+      have ⟨_, _, h₁⟩ := ih₁ (hnz := hnz) haff₁ hmem₁ hmem₁
+      have ⟨_, _, h₂⟩ := ih₂ (hnz := hnz) haff₂ hmem₂ hmem₂
+      exact False.elim (hdisj h₁ h₂)
+    · rename_i hmem₁ hmem₂
+      have := ih₂ (hnz := hnz) haff₂ hmem₁ hmem₂
+      simp [ih₂ (hnz := hnz) haff₂ hmem₁ hmem₂]
+
 /-- `compileFn` preserves `AffineInrOp`. -/
 theorem compile_fn_preserves_aff_op
   [Arity Op₁] [Arity Op₂]
@@ -69,7 +149,14 @@ theorem compile_fn_preserves_aff_op
   {fn : Fn (Op₁ ⊕ Op₂) χ V m n}
   (haff : fn.AffineInrOp)
   : (compileFn hnz fn).AffineInrOp
-  := sorry
+  := by
+  have ⟨used, haff_body⟩ := haff
+  have : (compileFn.bodyComp hnz fn).AffineInrOp used
+    := compile_expr_preserves_aff_op haff_body
+  simp [compileFn, compileFn.initCarry, compileFn.resultSteers,
+    Proc.AffineInrOp]
+  simp [AtomicProcs.AffineInrOp] at this
+  grind only
 
 theorem map_chans_preserves_aff_op
   [Arity Op₁] [Arity Op₂]
@@ -90,6 +177,6 @@ theorem map_chans_preserves_aff_op
   subst h₁'
   simp at h₂ h₃ h₂' h₃'
   subst h₂ h₃ h₂' h₃'
-  simp [haff _ _ _ _ _ hmem_ap hmem_ap']
+  simp [haff hmem_ap hmem_ap']
 
 end Wavelet.Compile
